S2I/Examples/Increment.v
@@ -6,4 +6,4 @@ Require Import Source.Examples.Increment.
 Definition fuel := 1000%nat.
 Definition to_run := compile_and_run increment fuel.
 
-Extraction "/tmp/run_compiled_increment.ml" to_run.
+Extraction "/tmp/run_intermediate_compiled_increment.ml" to_run.
