Source/Examples/DefaultInitBuffer.v
@@ -21,4 +21,4 @@ Definition default_init_buffer: program := {|
 Definition fuel := 1000.
 Definition to_run := run default_init_buffer fuel.
 
-Extraction "/tmp/run_default_init_buffer.ml" to_run.
+Extraction "/tmp/run_source_default_init_buffer.ml" to_run.
