run_extracted_examples.sh
@@ -1,0 +1,34 @@
+#!/bin/bash
+
+EXAMPLES_DIR=Source/Examples
+EXTRACTION_DIR=/tmp
+
+SOURCE_PREFIX="run_source_"
+INTERMEDIATE_PREFIX="run_intermediate_compiled_"
+
+if (( $# == 1 )); then
+    if [[ $1 = "--force-extraction" ]]; then
+        echo "*** Forcing extraction ***"
+        touch $EXAMPLES_DIR/*.v
+        make
+    fi
+fi
+
+# run source examples
+echo "*** Running examples at the source level ***"
+for example in $EXTRACTION_DIR/$SOURCE_PREFIX*.ml; do
+    # prepend big int import to each example
+    echo -e "#load \"nums.cma\";;open Big_int;;\n$(cat $example)" > $example
+    # run the example
+    echo "Output of $example:"
+    ocaml $example
+done
+
+# run compiled examples at the intermediate level
+echo "*** Examples compiled at the intermediate level ***"
+for example in $EXTRACTION_DIR/$INTERMEDIATE_PREFIX*.ml; do
+    # prepend big int import to each example
+    echo -e "#load \"nums.cma\";;open Big_int;;\n$(cat $example)" > $example
+    echo "Output of $example:"
+    ocaml $example
+done
